[[!4.3 Boolean Algebra]]

## De Morgan's Law

- **Complex expressions** can be made **simpler** using the rules of **Boolean algebra**
    
- This is a **more powerful simplification** method than Karnaugh maps and can simplify expressions that Karnaugh maps cannot
    
- There are various different **rules** that you need to learn and that can then be applied to certain expressions to simplify them
    
- **Combining these rules** can mean that c**omplex expressions** can be **reduced to much simpler ones**
    

### General rules

**General AND rules**

- X AND 0 = 0
    
- X AND 1 = X
    
- X AND A = X
    
- NOT X AND X = 0
    

Note, the value ox X is unknown and it is used as a placeholder. Therefore **X AND 1 = X** means that the output will be whatever the value of X is. 

**General OR rules**

- X OR 0 = X  
    X OR 1 = 1  
    X OR A = X  
    NOT X OR X = 1
    

### DeMorgan's Law

- This provides a strategy for simplifying expressions that include a negation of a conjunction or disjunction (simplifying by inverting all variable)
    
- **NOT(A AND B)** is the same as (**NOT A) OR (NOT B)**
    

![DeMorgan's Law](https://cdn.savemyexams.com/cdn-cgi/image/f=auto,width=3840/https://cdn.savemyexams.com/uploads/2024/04/screenshot-2024-04-02-at-2-32-45-pm.png)

- **Step 1**
    
    - Change AND to OR (or vice versa) - **¬(A V B)**
        
- **Step 2**
    
    - NOT the terms either side of the operator - **¬(¬A V ¬B)**
        
- **Step 3**
    
    - NOT everything that has changed -  **¬¬(¬A V ¬B)**
        
- **Step 4**
    
    - Get rid of any double negation -  **(¬A V ¬B)**
        
- **Step 5**
    
    - Remove any unnecessary brackets - **¬A V ¬B**
        

- **NOT(A OR B)** is the same as (**NOT A) AND (NOT B)**
    

![DeMorgan's Law](https://cdn.savemyexams.com/cdn-cgi/image/f=auto,width=3840/https://cdn.savemyexams.com/uploads/2024/04/screenshot-2024-04-02-at-2-33-06-pm.png)

- **Step 1**
    
    - Change AND to OR (or vice versa) - **¬(A ^ B)**
        
- **Step 2**
    
    - NOT the terms either side of the operator - **¬(¬A ^ ¬B)**
        
- **Step 3**
    
    - NOT everything that has changed -  **¬¬(¬A ^ ¬B)**
        
- **Step 4**
    
    - Get rid of any double negation -  **(¬A ^ ¬B)**
        
- **Step 5**
    
    - Remove any unnecessary brackets - **¬A ^ ¬B**
        
- Simplifying using this law allows the use of **only NAND or NOR gates** which makes **building microprocessors** much **easier** (i.e. Flash drives)
    

## Distribution

### Distributive Law

- This explains how AND and OR interact with each other
    
- This is a bit like factorising in normal maths
    
- **A AND (B OR C)** is the same as **(A AND B) OR (A AND C)**
    
- **A OR (B AND C)** is the same as **(A OR B) AND (A OR C**
    

**Real-life example**

- "_You can pick one subject from group A and either one from group B or group C_"
    
- is the same as
    
- "_You can pick one subject from group A and one from group B or one subject from group A and one from group C_"
    

## Association

### Associative Law

- This explains how variables associate in expressions of more than two variables
    
- Allows us to remove brackets and regroup variables
    
- **(A AND B) AND C** is the same as **A AND (B AND C)** is the same as **A AND B AND C**
    
- **(A OR B) OR C** is the same as **A OR (B OR C)** is the same as **A OR B OR C**
    

**Real-life example**

- "_Zarmeen and her friends, Zahra and Ella have been chosen to represent the school"_
    
- is the same as
    
- _"Zarmeen and Zahra, and their friend Ella have been chosen to represent the school"_
    
- is the same as
    
- _"Zarmeen, Zahra and Ella have been chosen to the represent the school"_
    

## Commutation

### Commutative Law

- States that the order of the variables does not change the truth value of the expression
    
- **A AND B** is the same as **B AND A**
    
- **A OR B** is the same as **B OR A**
    

**Real-life example**

- "_Fynn and George won gold medals"_
    
- is the same as
    
- _George and Fynn won gold medals"_
    

## Double Negation

### Double Negation Law

- States that the double negation of a variable results in the original variable
    
- NOT(NOT(A)) = A
    

**Real-life example**

- "_I don't not want to visit the castle"_
    
- is the same as 
    
- _"I do want to visit the castle"_
    

#### Worked Example

### SIMPLIFYING EXPRESSION EXAMPLE

**Simplify (A v B) ^ (A v C)**

**How to answer this question:**

**Step one - Distribution**  
This is a bit like multiplying out the brackets in an expression in regular maths. Think of OR being like ADD and AND being like MULTIPLY.

(A v B) ^ (A v C)   
becomes  
(A ^ A) v (B ^ A) v (A ^ C) v (B ^ C)

**Step two - General rules**  
Since (A ^ A) is just A we can replace this term in the expression with a simpler one.

(A ^ A) v (B ^ A) v (A ^ C) v (B ^ C)   
becomes  
A v (B ^ A) v (A ^ C) v (B ^ C)

**Step three - Commutation**  
This means the order of the logical operators does not matter so can change (B ^ A) into (A ^ B).

 A v (B ^ A) v (A ^ C) v (B ^ C)   
becomes  
A v (A ^ B) v (A ^ C) v (B ^ C)

**Step four - Absorption**  
This rule says that A AND (A OR B) = A.

A v (A ^ B) v (A ^ C) v (B ^ C)   
becomes  
A v (A ^ C) v (B ^ C)

**Step five - Another absorption**  
Again this rule says that A AND (A OR C) = A so

 A v (A ^ C) v (B ^ C)   
becomes  
A v (B ^ C)

**Example answer that gets full marks:**

A v (B ^ C)